Init commit, adding i1 to Compiler

src/coq/Compiler.v
@@ -19,6 +19,16 @@ Require Import Vellvm.Classes Vellvm.Ollvm_ast Vellvm.AstLib.
 (* Logical Foundations dependencies *)
 Require Import Vellvm.Imp Vellvm.Maps.
 
+(* Setup for 1bit integers *)
+Module Wordsize1.
+  Definition wordsize := 1%nat.
+  Remark wordsize_not_zero: wordsize <> 0%nat.
+  Proof. unfold wordsize; congruence. Qed.
+End Wordsize1.
+
+Module Int1 := Make(Wordsize1).
+
+Definition int1 := Int1.int.
 
 (* "Flattened" representation of Vellvm code *)
 Inductive elt :=
@@ -197,6 +207,9 @@ Definition val_of_nat (n:nat) : value :=
 Definition val_of_int64 (i:int64) : value :=
   SV (VALUE_Integer (Int64.signed i)).
 
+Definition val_of_int1 (i:int1) : value :=
+  SV (VALUE_Integer (Int1.signed i)).
+
 Definition val_of_ident (id:ident) : value :=
   SV (VALUE_Ident id).
 
@@ -272,19 +285,19 @@ Fixpoint compile_bexp (g:ctxt) (b:bexp) : LLVM value :=
       mret (local lid)
   in
   match b with
-  | BTrue     => (* TO SEE: CHKoh: mret (val_of_bool true) *)
-    'lid <- comp Eq (val_of_int64 (Int64.repr 0)) (val_of_int64 (Int64.repr 0));
+  | BTrue     => 
+    'lid <- comp Eq (val_of_int1 (Int1.repr 0)) (val_of_int1 (Int1.repr 0));
     mret (local lid)
-  | BFalse    => (* TO SEE: CHKoh: mret (val_of_bool false) *)
-    'lid <- comp Eq (val_of_int64 (Int64.repr 1)) (val_of_int64 (Int64.repr 0));
+  | BFalse    => 
+    'lid <- comp Eq (val_of_int1 (Int1.repr 1)) (val_of_int1 (Int1.repr 0));
     mret (local lid)
   | BEq a1 a2 => compile_icmp Eq a1 a2
   | BLe a1 a2 => compile_icmp Ule a1 a2
   | BNot b =>
     'v <- compile_bexp g b;
       (* TO SEE: CHKoh: 'lid <- binop Xor i1 v (val_of_bool true); *)
-    (*!*) 't <- comp Eq (val_of_int64 (Int64.repr 0)) (val_of_int64 (Int64.repr 0));
-    (*! 't <- comp Eq (val_of_int64 (Int64.repr 1)) (val_of_int64 (Int64.repr 0)); *)
+    (*!*) 't <- comp Eq (val_of_int1 (Int1.repr 0)) (val_of_int1 (Int1.repr 0));
+    (*! 't <- comp Eq (val_of_int1 (Int1.repr 1)) (val_of_int1 (Int1.repr 0)); *)
     'lid <- binop Xor i1 v (local t);
     mret (local lid) 
 
