src/coq/ImpCorrectness.v
@@ -1090,3 +1090,317 @@ Lemma compile_bexp_correct :
         (slc_pc fn bid phis term (List.rev c_a), e, k) mem.
 Proof.
 Admitted.
+  (*
+intros a st ans HAexp.
+  rewrite aeval_iff_aevalR in HAexp.
+
+  induction HAexp; intros g n m cd n' m' cd' v Hcomp.
+  - simpl in Hcomp. unfold_llvm Hcomp. simpl in Hcomp.
+    inversion Hcomp. clear Hcomp.
+    exists [I (IId (lid_of_Z n))
+         (INSTR_Op (SV (OP_IBinop (Add false false) i1 (val_of_int1 ans) (val_of_int1 Integers.Int1.zero))))].
+    exists [((IId (lid_of_Z n)),
+         (INSTR_Op (SV (OP_IBinop (Add false false) i1 (val_of_int1 ans) (val_of_int1 Integers.Int1.zero)))))].
+    repeat split; auto.
+    * repeat econstructor.
+    
+    * intros e mem Hlt HM k CFG fn0 bid phis term. 
+      eapply step_tau; auto.
+      apply pc_prefix_id.
+      simpl.
+    eapply step_zero. repeat split; auto.
+    + eapply memory_invariant_extension; eauto; try omega.
+    + unfold eval_expr.  simpl. rewrite lookup_env_hd.
+      repeat rewrite Int1.repr_signed. rewrite Int1.add_zero. auto.
+    + eapply env_extends_lt. apply Hlt. 
+    + apply env_lt_cons. omega. eapply env_lt_weaken; eauto. omega.
+
+  - simpl in Hcomp. unfold_llvm Hcomp.
+    unfold trywith in Hcomp.
+    remember (g id) as X.
+    destruct X; simpl in Hcomp; try inversion Hcomp.
+    clear Hcomp.
+    exists [I (IId (lid_of_Z n)) (INSTR_Load false i1 (i1ptr, v0) None)].
+    exists [(IId (lid_of_Z n), (INSTR_Load false i1 (i1ptr, v0) None))].
+    simpl. repeat split; auto.
+    * apply straight_Eff; auto. econstructor.
+    * intros e mem Hlt HM k CFG fn0 bid phis term.
+     destruct HM with (x:=id)(v:=v0) as [n1 [Hlt1 [a [Hlookup HRa]]]]; auto.
+     eapply step_eff; auto.
+    + apply pc_prefix_id.
+    + subst; simpl; unfold eval_expr; simpl; rewrite Hlookup; simpl;  eauto.
+    + simpl. eauto.
+    + eapply step_zero.
+      repeat split; auto.
+      -- eapply memory_invariant_extension; eauto. 
+      -- unfold eval_expr; simpl; rewrite lookup_env_hd; auto.
+      -- eapply env_extends_lt; eauto. 
+      -- apply env_lt_cons. omega. eapply env_lt_weaken; eauto. omega.
+        
+  - simpl in Hcomp;
+    unfold_llvm Hcomp;
+    specialize IHHAexp1 with (g:=g)(n:=n)(m:=m)(cd:=cd).
+    remember (compile_aexp g a1 (n, m, cd)) as f.
+    destruct f as [[[n1 m1] cd1] [err1|v1]];
+    try solve [inversion Hcomp].
+    specialize IHHAexp1 with (n':=n1)(m':=m1)(cd':=cd1)(v:=v1).
+    lapply IHHAexp1; clear IHHAexp1; [intros IHHAexp1 | auto].
+    destruct IHHAexp1 as [cd_a1 [c_a1 [Hcd_eq1 [Hcc1 [HSlc1 IHHAexp1]]]]].
+
+    symmetry in Heqf;
+    apply compile_aexp_monotonic in Heqf;
+    destruct Heqf as [ltn1 [ltm1 [cd1' Heq_cd1]]].
+
+    
+    specialize IHHAexp2 with (g:=g)(n:=n1)(m:=m1)(cd:=cd1).
+    remember (compile_aexp g a2 (n1, m1, cd1)) as f2;
+    destruct f2 as [[[n2 m2] cd2] [err2|v2]];
+    try solve [inversion Hcomp].
+    specialize IHHAexp2 with (n':=n2)(m':=m2)(cd':=cd2)(v:=v2).
+    lapply IHHAexp2; clear IHHAexp2; [intros IHHAexp2 | auto].
+    destruct IHHAexp2 as [cd_a2 [c_a2 [Hcd_eq2 [Hcc2 [HSlc2 IHHAexp2]]]]].
+
+    symmetry in Heqf2;
+    apply compile_aexp_monotonic in Heqf2;
+    destruct Heqf2 as [ltn2 [ltm2 [cd2' Heq_cd2]]].
+
+
+    simpl in Hcomp.
+    inversion Hcomp. clear Hcomp.
+
+    subst.
+    exists (I (IId (lid_of_Z n2)) (INSTR_Op (SV (OP_IBinop (Add false false) i1 v1 v2)))::cd2' ++ cd1').
+    exists (((IId (lid_of_Z n2)),(INSTR_Op (SV (OP_IBinop (Add false false) i1 v1 v2))))::c_a2 ++ c_a1).
+    simpl. repeat split; auto.
+    + rewrite app_assoc. reflexivity.
+    + apply cc_cons_Op. apply compiled_code_app; auto.
+      apply app_inv_tail in Hcd_eq2. rewrite Hcd_eq2. auto.
+      apply app_inv_tail in Hcd_eq1. rewrite Hcd_eq1. auto.
+    + apply straight_Op; auto. apply straight_app; auto.
+    + intros e mem Hlt Hmem k CFG fn bid phis term.
+      rewrite rev_app_distr.
+      specialize IHHAexp1 with (e:=e)(mem:=mem).
+      lapply IHHAexp1; clear IHHAexp1; [intros IHHAexp1 | auto].
+      lapply IHHAexp1; clear IHHAexp1; [intros IHHAexp1 | auto].
+      specialize IHHAexp1 with (k:=k)(CFG:=CFG)(fn:=fn)(bid:=bid)(phis:=phis)(term:=term).
+
+      rewrite <- app_assoc.
+      eapply step_code_app. apply IHHAexp1. clear IHHAexp1.
+      intros st1 mem1 H. 
+      destruct st1 as [[pc1 e1] k1].
+      destruct H as [Hpc1 [Hmem1 [Hr1 [He1 Hlte1]]]].
+      split; subst; auto.
+
+      specialize IHHAexp2 with (e:=e1)(mem:=mem1).
+      lapply IHHAexp2; clear IHHAexp2; [intros IHHAexp2 | auto].
+      lapply IHHAexp2; clear IHHAexp2; [intros IHHAexp2 | auto].
+      specialize IHHAexp2 with (k:=k1)(CFG:=CFG)(fn:=fn)(bid:=bid)(phis:=phis)(term:=term).
+
+      simpl.
+      rewrite pc_app_slc. simpl.
+      eapply step_code_app.
+      apply IHHAexp2.
+      intros st2 mem2 H2.
+      destruct st2 as [[pc2 e2] k2].
+      destruct H2 as [Hpc2 [Hmem2 [Hr2 [He2 Hlte2]]]].
+      split; subst; auto.
+      
+      eapply step_tau; auto.
+      * simpl. unfold pc_app. simpl. apply pc_prefix_id.
+      * simpl.
+        inversion Hr1. subst. inversion Hr2. subst.
+        symmetry in H.
+        assert (eval_op e2 (Some (TYPE_I 1)) v1 = inr v).
+        apply He2; auto.
+        simpl.
+        unfold eval_expr. simpl. unfold i1.
+        rewrite H3. rewrite <- H1. simpl.
+        inversion H0. inversion H2. simpl.
+        eauto.
+      * simpl. eapply step_zero.
+        repeat split; auto.
+        ++ eapply memory_invariant_extension; eauto. 
+        ++ unfold eval_expr; simpl; rewrite lookup_env_hd; auto.
+        ++ eapply env_extends_trans. apply He1.
+           eapply env_extends_trans. apply He2.
+           eapply env_extends_lt. apply Hlte2. 
+        ++ apply env_lt_cons. omega. eapply env_lt_weaken; eauto. omega.
+
+  - simpl in Hcomp;
+    unfold_llvm Hcomp;
+    specialize IHHAexp1 with (g:=g)(n:=n)(m:=m)(cd:=cd).
+    remember (compile_aexp g a1 (n, m, cd)) as f;
+    destruct f as [[[n1 m1] cd1] [err1|v1]];
+    try solve [inversion Hcomp].
+    specialize IHHAexp1 with (n':=n1)(m':=m1)(cd':=cd1)(v:=v1).
+    lapply IHHAexp1; clear IHHAexp1; [intros IHHAexp1 | auto].
+    destruct IHHAexp1 as [cd_a1 [c_a1 [Hcd_eq1 [Hcc1 [HSlc1 IHHAexp1]]]]].
+
+    symmetry in Heqf;
+    apply compile_aexp_monotonic in Heqf;
+    destruct Heqf as [ltn1 [ltm1 [cd1' Heq_cd1]]].
+
+    
+    specialize IHHAexp2 with (g:=g)(n:=n1)(m:=m1)(cd:=cd1).
+    remember (compile_aexp g a2 (n1, m1, cd1)) as f2;
+    destruct f2 as [[[n2 m2] cd2] [err2|v2]];
+    try solve [inversion Hcomp].
+    specialize IHHAexp2 with (n':=n2)(m':=m2)(cd':=cd2)(v:=v2).
+    lapply IHHAexp2; clear IHHAexp2; [intros IHHAexp2 | auto].
+    destruct IHHAexp2 as [cd_a2 [c_a2 [Hcd_eq2 [Hcc2 [HSlc2 IHHAexp2]]]]].
+
+    symmetry in Heqf2;
+    apply compile_aexp_monotonic in Heqf2;
+    destruct Heqf2 as [ltn2 [ltm2 [cd2' Heq_cd2]]].
+
+
+    simpl in Hcomp.
+    inversion Hcomp. clear Hcomp.
+
+    subst.
+    exists (I (IId (lid_of_Z n2)) (INSTR_Op (SV (OP_IBinop (Sub false false) i1 v1 v2)))::cd2' ++ cd1').
+    exists (((IId (lid_of_Z n2)),(INSTR_Op (SV (OP_IBinop (Sub false false) i1 v1 v2))))::c_a2 ++ c_a1).
+    simpl. repeat split; auto.
+    + rewrite app_assoc. reflexivity.
+    + apply cc_cons_Op. apply compiled_code_app; auto.
+      apply app_inv_tail in Hcd_eq2. rewrite Hcd_eq2. auto.
+      apply app_inv_tail in Hcd_eq1. rewrite Hcd_eq1. auto.
+    + apply straight_Op; auto. apply straight_app; auto.
+    + intros e mem Hlt Hmem k CFG fn bid phis term.
+      rewrite rev_app_distr.
+      specialize IHHAexp1 with (e:=e)(mem:=mem).
+      lapply IHHAexp1; clear IHHAexp1; [intros IHHAexp1 | auto].
+      lapply IHHAexp1; clear IHHAexp1; [intros IHHAexp1 | auto].
+      specialize IHHAexp1 with (k:=k)(CFG:=CFG)(fn:=fn)(bid:=bid)(phis:=phis)(term:=term).
+
+      rewrite <- app_assoc.
+      eapply step_code_app. apply IHHAexp1. clear IHHAexp1.
+      intros st1 mem1 H. 
+      destruct st1 as [[pc1 e1] k1].
+      destruct H as [Hpc1 [Hmem1 [Hr1 [He1 Hlte1]]]].
+      split; subst; auto.
+
+      specialize IHHAexp2 with (e:=e1)(mem:=mem1).
+      lapply IHHAexp2; clear IHHAexp2; [intros IHHAexp2 | auto].
+      lapply IHHAexp2; clear IHHAexp2; [intros IHHAexp2 | auto].
+      specialize IHHAexp2 with (k:=k1)(CFG:=CFG)(fn:=fn)(bid:=bid)(phis:=phis)(term:=term).
+
+      simpl.
+      rewrite pc_app_slc. simpl.
+      eapply step_code_app.
+      apply IHHAexp2.
+      intros st2 mem2 H2.
+      destruct st2 as [[pc2 e2] k2].
+      destruct H2 as [Hpc2 [Hmem2 [Hr2 [He2 Hlte2]]]].
+      split; subst; auto.
+      
+      eapply step_tau; auto.
+      * simpl. unfold pc_app. simpl. apply pc_prefix_id.
+      * simpl.
+        inversion Hr1. subst. inversion Hr2. subst.
+        symmetry in H.
+        assert (eval_op e2 (Some (TYPE_I 1)) v1 = inr v).
+        apply He2; auto.
+        simpl.
+        unfold eval_expr. simpl. unfold i1.
+        rewrite H3. rewrite <- H1. simpl.
+        inversion H0. inversion H2. simpl.
+        eauto.
+      * simpl. eapply step_zero.
+        repeat split; auto.
+        ++ eapply memory_invariant_extension; eauto. 
+        ++ unfold eval_expr; simpl; rewrite lookup_env_hd; auto.
+        ++ eapply env_extends_trans. apply He1.
+           eapply env_extends_trans. apply He2.
+           eapply env_extends_lt. apply Hlte2. 
+        ++ apply env_lt_cons. omega. eapply env_lt_weaken; eauto. omega.
+
+  - simpl in Hcomp;
+    unfold_llvm Hcomp;
+    specialize IHHAexp1 with (g:=g)(n:=n)(m:=m)(cd:=cd).
+    remember (compile_aexp g a1 (n, m, cd)) as f;
+    destruct f as [[[n1 m1] cd1] [err1|v1]];
+    try solve [inversion Hcomp].
+    specialize IHHAexp1 with (n':=n1)(m':=m1)(cd':=cd1)(v:=v1).
+    lapply IHHAexp1; clear IHHAexp1; [intros IHHAexp1 | auto].
+    destruct IHHAexp1 as [cd_a1 [c_a1 [Hcd_eq1 [Hcc1 [HSlc1 IHHAexp1]]]]].
+
+    symmetry in Heqf;
+    apply compile_aexp_monotonic in Heqf;
+    destruct Heqf as [ltn1 [ltm1 [cd1' Heq_cd1]]].
+
+    
+    specialize IHHAexp2 with (g:=g)(n:=n1)(m:=m1)(cd:=cd1).
+    remember (compile_aexp g a2 (n1, m1, cd1)) as f2;
+    destruct f2 as [[[n2 m2] cd2] [err2|v2]];
+    try solve [inversion Hcomp].
+    specialize IHHAexp2 with (n':=n2)(m':=m2)(cd':=cd2)(v:=v2).
+    lapply IHHAexp2; clear IHHAexp2; [intros IHHAexp2 | auto].
+    destruct IHHAexp2 as [cd_a2 [c_a2 [Hcd_eq2 [Hcc2 [HSlc2 IHHAexp2]]]]].
+
+    symmetry in Heqf2;
+    apply compile_aexp_monotonic in Heqf2;
+    destruct Heqf2 as [ltn2 [ltm2 [cd2' Heq_cd2]]].
+
+
+    simpl in Hcomp.
+    inversion Hcomp. clear Hcomp.
+
+    subst.
+    exists (I (IId (lid_of_Z n2)) (INSTR_Op (SV (OP_IBinop (Mul false false) i1 v1 v2)))::cd2' ++ cd1').
+    exists (((IId (lid_of_Z n2)),(INSTR_Op (SV (OP_IBinop (Mul false false) i1 v1 v2))))::c_a2 ++ c_a1).
+    simpl. repeat split; auto.
+    + rewrite app_assoc. reflexivity.
+    + apply cc_cons_Op. apply compiled_code_app; auto.
+      apply app_inv_tail in Hcd_eq2. rewrite Hcd_eq2. auto.
+      apply app_inv_tail in Hcd_eq1. rewrite Hcd_eq1. auto.
+    + apply straight_Op; auto. apply straight_app; auto.
+    + intros e mem Hlt Hmem k CFG fn bid phis term.
+      rewrite rev_app_distr.
+      specialize IHHAexp1 with (e:=e)(mem:=mem).
+      lapply IHHAexp1; clear IHHAexp1; [intros IHHAexp1 | auto].
+      lapply IHHAexp1; clear IHHAexp1; [intros IHHAexp1 | auto].
+      specialize IHHAexp1 with (k:=k)(CFG:=CFG)(fn:=fn)(bid:=bid)(phis:=phis)(term:=term).
+
+      rewrite <- app_assoc.
+      eapply step_code_app. apply IHHAexp1. clear IHHAexp1.
+      intros st1 mem1 H. 
+      destruct st1 as [[pc1 e1] k1].
+      destruct H as [Hpc1 [Hmem1 [Hr1 [He1 Hlte1]]]].
+      split; subst; auto.
+
+      specialize IHHAexp2 with (e:=e1)(mem:=mem1).
+      lapply IHHAexp2; clear IHHAexp2; [intros IHHAexp2 | auto].
+      lapply IHHAexp2; clear IHHAexp2; [intros IHHAexp2 | auto].
+      specialize IHHAexp2 with (k:=k1)(CFG:=CFG)(fn:=fn)(bid:=bid)(phis:=phis)(term:=term).
+
+      simpl.
+      rewrite pc_app_slc. simpl.
+      eapply step_code_app.
+      apply IHHAexp2.
+      intros st2 mem2 H2.
+      destruct st2 as [[pc2 e2] k2].
+      destruct H2 as [Hpc2 [Hmem2 [Hr2 [He2 Hlte2]]]].
+      split; subst; auto.
+      
+      eapply step_tau; auto.
+      * simpl. unfold pc_app. simpl. apply pc_prefix_id.
+      * simpl.
+        inversion Hr1. subst. inversion Hr2. subst.
+        symmetry in H.
+        assert (eval_op e2 (Some (TYPE_I 1)) v1 = inr v).
+        apply He2; auto.
+        simpl.
+        unfold eval_expr. simpl. unfold i1.
+        rewrite H3. rewrite <- H1. simpl.
+        inversion H0. inversion H2. simpl.
+        eauto.
+      * simpl. eapply step_zero.
+        repeat split; auto.
+        ++ eapply memory_invariant_extension; eauto. 
+        ++ unfold eval_expr; simpl; rewrite lookup_env_hd; auto.
+        ++ eapply env_extends_trans. apply He1.
+           eapply env_extends_trans. apply He2.
+           eapply env_extends_lt. apply Hlte2. 
+        ++ apply env_lt_cons. omega. eapply env_lt_weaken; eauto. omega.
+Qed.*)
